Supposed to be easy: encrypt for chachapoly

providers/evercrypt/EverCrypt.AEAD.fsti
@@ -1,5 +1,15 @@
 module EverCrypt.AEAD
 
+/// The new AEAD interface for EverCrypt, which supersedes the functions found
+/// in EverCrypt.fst
+///
+/// The expected usage for this module is as follows:
+/// - client expands key, obtaining an ``expanded_key a``
+/// - client uses ``encrypt``/``decrypt`` with the same ``expanded_key a`` repeatedly.
+///
+/// This usage protocol is enforced for verified F* clients but, naturally,
+/// isn't for C clients.
+
 module S = FStar.Seq
 module G = FStar.Ghost
 
@@ -13,23 +23,54 @@ open FStar.Integers
 
 open Spec.AEAD
 
+/// Note: if the fst and the fsti are running on different fuel settings,
+/// something that works in the interactive mode for the fsti, when
+/// "re-interpreted" in the fst, might stop working!
+#set-options "--max_fuel 0 --max_ifuel 0"
+
 noextract
 let bytes = Seq.seq UInt8.t
 
 let frozen_preorder (s: bytes): MB.srel UInt8.t = fun (s1 s2: bytes) ->
   S.equal s1 s ==> S.equal s2 s
 
+/// We need to be able to return a proper ``expanded_key`` even if the algorithm
+/// is unsupported, so that C clients don't trip this interface. Alternatively,
+/// we could remove this layer of complexity and let C clients get a fatal
+/// kremlin abort if they try to use AEAD for an unsupported algorithm (see
+/// 486790f5).
+let kv_or_dummy (a: alg) = if is_supported_alg a then kv a else bytes
+
+let expand_or_dummy (a: alg) (kv: G.erased (kv_or_dummy a)) =
+  if is_supported_alg a then
+    // JP: I regularly have to perform let-bindings for these refinement types to work
+    let a = a in
+    expand #a (G.reveal kv)
+  else
+    S.empty
+
+/// This type, following several rounds of optimization by KreMLin, will extract
+/// to a regular pointer type. A NULL pointer indicates an invalid expanded key.
 noeq
-type expanded_key (a: supported_alg) =
+type expanded_key (a: alg) =
 | EK:
-    kv:G.erased (kv a) -> ek:(
-    let s = expand (G.reveal kv) in
+    kv:G.erased (kv_or_dummy a) ->
+    ek:(
+    [@ inline_let ]
+    let s = expand_or_dummy a kv in
+    [@ inline_let ]
     let p = frozen_preorder s in
-    ek:MB.mbuffer UInt8.t p p { MB.witnessed ek (S.equal s) }) ->
+    ek:MB.mbuffer UInt8.t p p { not (MB.g_is_null ek) ==> MB.witnessed ek (S.equal s) }) ->
     expanded_key a
 
+/// When successful, this function returns a non-NULL pointer that has been
+/// freshly allocated and that contains the expanded key.
+///
+/// Possible causes for a NULL pointer include:
+/// - unsupported algorithm
+/// - unavailable implementation on target platform
 val expand_in:
-  #a:supported_alg ->
+  #a:alg ->
   r:HS.rid ->
   k:B.buffer UInt8.t { B.length k = key_length a } ->
   ST (expanded_key a)
@@ -41,33 +82,59 @@ val expand_in:
       Hash.fresh_loc l h0 h1 /\
       B.(modifies loc_none h0 h1) /\
       B.(loc_includes (loc_region_only true r) l) /\
-      S.equal (G.reveal (EK?.kv ek)) (B.as_seq h0 k))
+      (not (MB.g_is_null (EK?.ek ek)) ==> (
+        S.equal (G.reveal (EK?.kv ek)) (B.as_seq h0 k) /\
+        is_supported_alg a)))
 
 let iv_p a = iv:B.buffer UInt8.t { B.length iv = iv_length a }
 let ad_p a = ad:B.buffer UInt8.t { B.length ad <= max_length a }
 let plain_p a = p:B.buffer UInt8.t { B.length p <= max_length a }
 
+type error_code =
+| Success
+| InvalidKey
+| Failure
+
+let _: squash (inversion error_code) = allow_inversion error_code
+
+/// This function takes a previously expanded key and performs encryption.
+///
+/// Possible return values are:
+/// - ``Success``: encryption was successfully performed
+/// - ``InvalidKey``: the function was passed a NULL expanded key (see above)
+/// ``Failure`` is currently unused but may be used in the future.
 val encrypt:
   #a:supported_alg ->
   ek:expanded_key a ->
   iv:iv_p a ->
   ad:ad_p a ->
-  ad_len: UInt32.t { v ad_len = B.length ad } ->
+  ad_len: UInt32.t { v ad_len = B.length ad /\ v ad_len <= pow2 31 } ->
   plain: plain_p a ->
-  plain_len: UInt32.t { v plain_len = B.length plain } ->
+  plain_len: UInt32.t { v plain_len = B.length plain /\ v plain_len <= max_length a } ->
   dst: B.buffer UInt8.t { B.length dst = B.length plain + tag_length a } ->
-  Stack unit
+  Stack error_code
     (requires fun h0 ->
-      B.live h0 (EK?.ek ek) /\
-      B.live h0 iv /\
-      B.live h0 ad /\
-      B.live h0 plain /\
-      B.live h0 dst)
-    (ensures fun h0 _ h1 ->
-      B.(modifies (loc_buffer dst) h0 h1) /\
-      S.equal (B.as_seq h1 dst)
-        (encrypt (G.reveal (EK?.kv ek)) (B.as_seq h0 iv) (B.as_seq h0 ad) (B.as_seq h0 plain)))
+      MB.(all_live h0 [ buf (EK?.ek ek); buf iv; buf ad; buf plain; buf dst ]) /\
+      (B.disjoint plain dst \/ plain == dst) /\
+      B.disjoint iv dst /\
+      B.disjoint ad dst)
+    (ensures fun h0 r h1 ->
+      match r with
+      | Success ->
+          B.(modifies (loc_buffer dst) h0 h1) /\
+          S.equal (B.as_seq h1 dst)
+            (encrypt #a (G.reveal (EK?.kv ek)) (B.as_seq h0 iv) (B.as_seq h0 ad) (B.as_seq h0 plain))
+      | InvalidKey ->
+          B.(modifies loc_none h0 h1)
+      | Failure ->
+        False)
 
+/// This function takes a previously expanded key and performs decryption.
+///
+/// Possible return values are:
+/// - ``Success``: decryption was successfully performed
+/// - ``InvalidKey``: the function was passed a NULL expanded key (see above)
+/// - ``Failure``: cipher text could not be decrypted (e.g. tag mismatch)
 val decrypt:
   #a:supported_alg ->
   ek:expanded_key a ->
@@ -77,18 +144,22 @@ val decrypt:
   cipher: plain_p a ->
   cipher_len: UInt32.t { v cipher_len = B.length cipher } ->
   dst: B.buffer UInt8.t { B.length dst = B.length cipher - tag_length a } ->
-  Stack bool
+  Stack error_code
     (requires fun h0 ->
       B.live h0 (EK?.ek ek) /\
       B.live h0 iv /\
       B.live h0 ad /\
       B.live h0 cipher /\
       B.live h0 dst)
-    (ensures fun h0 success h1 ->
-      B.(modifies (loc_buffer dst) h0 h1) /\ (
+    (ensures fun h0 err h1 ->
       let kv = G.reveal (EK?.kv ek) in
-      let plain = decrypt kv (B.as_seq h0 iv) (B.as_seq h0 ad) (B.as_seq h0 cipher) in
-      if success then
-        Some? plain /\ S.equal (Some?.v plain) (B.as_seq h1 dst)
-      else
-        None? plain))
+      let plain = decrypt #a kv (B.as_seq h0 iv) (B.as_seq h0 ad) (B.as_seq h0 cipher) in
+      match err with
+      | InvalidKey ->
+          B.(modifies loc_none h0 h1)
+      | Success ->
+          B.(modifies (loc_buffer dst) h0 h1) /\
+          Some? plain /\ S.equal (Some?.v plain) (B.as_seq h1 dst)
+      | Failure ->
+          B.(modifies (loc_buffer dst) h0 h1) /\
+          None? plain)
