providers/evercrypt/fst/EverCrypt.AEAD.fst
@@ -28,10 +28,13 @@ let expand_in #a r k =
   | AES128_GCM | AES256_GCM ->
       let h0 = ST.get () in
       let kv: G.erased (kv a) = G.hide (B.as_seq h0 k) in
-      let ek =
-        MB.mmalloc #UInt8.t #(frozen_preorder (expand #a (G.reveal kv))) r 0uy (ekv_len a)
-      in
-      admit () // waiting for interop wrappers
+      if EverCrypt.TargetConfig.x64 then
+        let ek =
+          MB.mmalloc #UInt8.t #(frozen_preorder (expand #a (G.reveal kv))) r 0uy (ekv_len a)
+        in
+        admit () // waiting for interop wrappers
+      else
+        EK kv MB.mnull
   | CHACHA20_POLY1305 ->
       let h0 = ST.get () in
       let kv: G.erased (kv a) = G.hide (B.as_seq h0 k) in
@@ -42,3 +45,33 @@ let expand_in #a r k =
       assert (B.as_seq h2 ek == B.as_seq h0 k);
       MB.witness_p ek (S.equal (G.reveal kv));
       EK kv ek
+  | _ ->
+      EK (G.hide (S.empty #UInt8.t)) MB.mnull
+
+#set-options "--z3rlimit 100"
+let encrypt #a ek iv ad ad_len plain plain_len dst =
+  if MB.is_null (EK?.ek ek) then
+    InvalidKey
+  else match a with
+  | AES128_GCM | AES256_GCM ->
+      admit ()
+  | CHACHA20_POLY1305 ->
+      // Monotonicity; gives us proper length for ek while we're at it.
+      MB.recall_p (EK?.ek ek) (S.equal (expand_or_dummy a (EK?.kv ek)));
+      assert (MB.length (EK?.ek ek) = 32);
+      assert (B.length iv = 12);
+
+      push_frame ();
+      // Cannot pass a frozen buffer to a function that expects a regular
+      // buffer. (Or can we? Prove compatibility of preorders?). In any case, we
+      // just allocate a temporary on the stack and blit.
+      let tmp = B.alloca 0uy 32ul in
+      MB.blit (EK?.ek ek) 0ul tmp 0ul 32ul;
+
+      // Length restrictions
+      assert_norm (pow2 31 + pow2 32 / 64 <= pow2 32 - 1);
+
+      Hacl.Impl.Chacha20Poly1305.aead_encrypt_chacha_poly
+        tmp iv ad_len ad plain_len plain dst;
+      pop_frame ();
+      Success
